Add join_assoc lemma

Classes/Joinable.v
@@ -6,6 +6,8 @@ Class Joinable (T : Type) `{PreorderedSet T} : Type :=
   join_op : T -> T -> T;
   join_upper_bound_left: forall t t', preorder t (join_op t t');
   join_upper_bound_right: forall t t', preorder t' (join_op t t');
+  join_assoc : ∀ x y z : T, 
+    join_op x (join_op y z) = join_op (join_op x y) z;
 }.
 Arguments join_op : simpl never.
 Hint Resolve join_upper_bound_left join_upper_bound_right : soundness.
